[repdb] more specs.

aneris/examples/reliable_communication/lib/repdb/spec/ras.v
@@ -12,18 +12,31 @@ Class DBG `{!DB_time, !DB_events} Σ :=
     DBG_Global_history_mono :>
       inG Σ (authUR (monotoneUR (@prefix (leibnizO we))));
     DBG_Local_history_mono :>
-      inG Σ (authUR (gmapUR socket_address
-                               (monotoneUR (@prefix (leibnizO we)))));
+      inG Σ (gmapUR socket_address (agreeR gnameO));
     DBG_lockG :>
       lockG Σ;
+    DBG_followers_gname : gname;
+
 }.
+
+Class DBPreG `{!DB_time, !DB_events} Σ :=
+  {
+    DBG_preGlobal_mem_excl :>
+      inG Σ (authUR (gmapUR Key (prodR fracR (agreeR (optionO (leibnizO we))))));
+    DBG_preGlobal_history_mono :>
+      inG Σ (authUR (monotoneUR (@prefix (leibnizO we))));
+    DBG_preLocal_history_mono :>
+      inG Σ (gmapUR socket_address (agreeR gnameO));
+    DBG_prelockG :>
+      lockG Σ;
+}.
+
 
 Definition DBΣ `{!DB_time, !DB_events} : gFunctors :=
   #[GFunctor (authUR (gmapUR Key (prodR fracR (agreeR (optionO (leibnizO we))))));
     GFunctor (authUR (monotoneUR (@prefix (leibnizO we))));
-    GFunctor (authUR (gmapUR socket_address
-                               (monotoneUR (@prefix (leibnizO we)))));
+    GFunctor (gmapUR socket_address (agreeR gnameO));
     lockΣ].
 
-Instance subG_DBΣ `{!DB_time, !DB_events, !lockG Σ} : subG DBΣ Σ → DBG Σ.
+Instance subG_DB_preGΣ `{!DB_time, !DB_events, !lockG Σ} : subG DBΣ Σ → DBPreG Σ.
 Proof. solve_inG. Qed.
